## circle
$(x-h)^2 + (y-k)^2 = r^2$
## ellipse
$\frac {(x-h)^2} {a^2} + \frac {(y-k)^2} {b^2} = 1$
or
$\frac {(y-k)^2} {a^2} + \frac {(x-h)^2} {b^2} = 1$
a != b
## parabola
$ax^2 + by$
or 
$ax + by^2$
## hyperbola
$\frac {(x-h)^2} {a^2} - \frac {(y-k)^2} {b^2} = 1$
or
$\frac {(y-k)^2} {a^2} - \frac {(x-h)^2} {b^2} = 1$


## circle vs ellipse
If you rearranged the circle to have an a and b value similar to an ellipse, the a and b values would be equivalent.

## ellipse vs hyperbola
An ellipse adds the two terms, while a hyperbola subtracts them.